@prefix dct: <http://purl.org/dc/terms/> .
@prefix owl: <http://www.w3.org/2002/07/owl#> .
@prefix rdf: <http://www.w3.org/1999/02/22-rdf-syntax-ns#> .
@prefix rdfs: <http://www.w3.org/2000/01/rdf-schema#> .
@prefix xs: <http://www.w3.org/2001/XMLSchema#> .

<http://purl.org/swan/2.0/discourse-relationships/>
	a owl:Ontology ;
	rdfs:label "Discourse relationships vocabulary v. 3.0" ;
	rdfs:comment "These relationships don't have range and domains defined as they are meant to be reused in different contexts" ;
	dct:contributor
		"David Shotton" ,
		"Elizabeth Wu" ,
		"Gwen Wong" ,
		"June Kinoshita" ,
		"Marco Ocana" ,
		"Paolo Ciccarese" ,
		"Tim Clark"
		;
	dct:creator <http://www.hcklab.org/foaf.rdf#me> ;
	dct:date "October 12, 2010" ;
	dct:format "rdf/xml" ;
	dct:language "en" ;
	dct:publisher "Massachusetts General Hospital" ;
	dct:title "Discourse relationships vocabulary"@en ;
	owl:versionInfo "3.0" ;
	.

dct:contributor
	a owl:AnnotationProperty ;
	.

dct:creator
	a owl:AnnotationProperty ;
	.

dct:date
	a owl:AnnotationProperty ;
	.

dct:format
	a owl:AnnotationProperty ;
	.

dct:language
	a owl:AnnotationProperty ;
	.

dct:publisher
	a owl:AnnotationProperty ;
	.

dct:title
	a owl:AnnotationProperty ;
	.

<http://purl.org/swan/2.0/discourse-relationships/alternativeTo>
	a
		owl:ObjectProperty ,
		owl:SymmetricProperty
		;
	rdfs:subPropertyOf <http://purl.org/swan/2.0/discourse-relationships/relatesTo> ;
	rdfs:label "alternativeTo" ;
	rdfs:comment """It connects two different resources that can be 
	    		considered alternative interpretations of the same experimental results""" ;
	.

<http://purl.org/swan/2.0/discourse-relationships/arisesFrom>
	a owl:ObjectProperty ;
	rdfs:subPropertyOf <http://purl.org/swan/2.0/discourse-relationships/refersTo> ;
	rdfs:label "arisesFrom" ;
	rdfs:comment "Something (question, doubt...) that arises because of something else" ;
	.

<http://purl.org/swan/2.0/discourse-relationships/consistentWith>
	a
		owl:ObjectProperty ,
		owl:SymmetricProperty
		;
	rdfs:subPropertyOf <http://purl.org/swan/2.0/discourse-relationships/relatesTo> ;
	rdfs:label "consistentWith" ;
	rdfs:comment """It expresses consistency between two resources. 
	    		It is a bidirectional relationship""" ;
	.

<http://purl.org/swan/2.0/discourse-relationships/inconsistentWith>
	a
		owl:ObjectProperty ,
		owl:SymmetricProperty
		;
	rdfs:subPropertyOf <http://purl.org/swan/2.0/discourse-relationships/relatesTo> ;
	rdfs:label "inconsistentWith" ;
	rdfs:comment """It expresses inconsistency between two resources. 
	    		It is a bidirectional relationship""" ;
	.

<http://purl.org/swan/2.0/discourse-relationships/motivates>
	a owl:ObjectProperty ;
	rdfs:subPropertyOf <http://purl.org/swan/2.0/discourse-relationships/refersTo> ;
	rdfs:label "motivates" ;
	rdfs:comment "Something (hypothesis, doubt...) that motivates something else like an experiment" ;
	.

<http://purl.org/swan/2.0/discourse-relationships/referencesAsInconsistentEvidence>
	a owl:ObjectProperty ;
	rdfs:subPropertyOf <http://purl.org/swan/2.0/discourse-relationships/refersTo> ;
	rdfs:label "referencesAsInconsistentEvidence" ;
	rdfs:comment "" ;
	.

<http://purl.org/swan/2.0/discourse-relationships/referencesAsRelevantEvidence>
	a owl:ObjectProperty ;
	rdfs:subPropertyOf <http://purl.org/swan/2.0/discourse-relationships/refersTo> ;
	rdfs:label "referencesAsRelevantEvidence" ;
	rdfs:comment "" ;
	.

<http://purl.org/swan/2.0/discourse-relationships/referencesAsSupportiveEvidence>
	a owl:ObjectProperty ;
	rdfs:subPropertyOf <http://purl.org/swan/2.0/discourse-relationships/refersTo> ;
	rdfs:label "referencesAsSupportiveEvidence" ;
	rdfs:comment "" ;
	.

<http://purl.org/swan/2.0/discourse-relationships/refersTo>
	a owl:ObjectProperty ;
	rdfs:subPropertyOf <http://purl.org/swan/2.0/discourse-relationships/relatesTo> ;
	rdfs:label "refersTo" ;
	rdfs:comment """It connects an entity with another entity in an 
				unidirectional way""" ;
	.

<http://purl.org/swan/2.0/discourse-relationships/relatesTo>
	a owl:ObjectProperty ;
	rdfs:label "relatesTo" ;
	rdfs:comment """The most generic relationship: it expresses connection 
			between two resources without specifying the nature of such connection""" ;
	.

<http://purl.org/swan/2.0/discourse-relationships/relevantTo>
	a
		owl:ObjectProperty ,
		owl:SymmetricProperty
		;
	rdfs:subPropertyOf <http://purl.org/swan/2.0/discourse-relationships/relatesTo> ;
	rdfs:label "relevantTo" ;
	rdfs:comment """It expresses the fact that a resource is 
	    		relevant for another one and vice-versa""" ;
	.

<http://purl.org/swan/2.0/discourse-relationships/respondsNegativelyTo>
	a owl:ObjectProperty ;
	rdfs:subPropertyOf <http://purl.org/swan/2.0/discourse-relationships/respondsTo> ;
	rdfs:label "respondsNegativelyTo" ;
	rdfs:comment """It expresses the fact that one entity is talking 
				    		about another one expressing disagreement""" ;
	.

<http://purl.org/swan/2.0/discourse-relationships/respondsNeutrallyTo>
	a owl:ObjectProperty ;
	rdfs:subPropertyOf <http://purl.org/swan/2.0/discourse-relationships/respondsTo> ;
	rdfs:label "respondsNeutrallyTo" ;
	rdfs:comment """It expresses the fact that one entity is 
				    		talking about another one without expressing agreement or disagreement""" ;
	.

<http://purl.org/swan/2.0/discourse-relationships/respondsPositivelyTo>
	a owl:ObjectProperty ;
	rdfs:subPropertyOf <http://purl.org/swan/2.0/discourse-relationships/respondsTo> ;
	rdfs:label "respondsPositivelyTo" ;
	rdfs:comment """It expresses the fact that one entity is talking 
				    		about another one expressing agreement""" ;
	.

<http://purl.org/swan/2.0/discourse-relationships/respondsTo>
	a owl:ObjectProperty ;
	rdfs:subPropertyOf <http://purl.org/swan/2.0/discourse-relationships/refersTo> ;
	rdfs:label "respondsTo" ;
	rdfs:comment "" ;
	.

