# imports: http://www.w3.org/2006/time#2016
# imports: http://www.w3.org/2006/vcard/ns
# imports: http://www.w3.org/ns/dcat
# imports: http://xmlns.com/foaf/0.1/
# imports: https://ontology.caseontology.org/case/case/1.1.0

@prefix case-corpora: <http://example.org/ontology/case-corpora/> .
@prefix dcat: <http://www.w3.org/ns/dcat#> .
@prefix dcterms: <http://purl.org/dc/terms/> .
@prefix foaf: <http://xmlns.com/foaf/0.1/> .
@prefix owl: <http://www.w3.org/2002/07/owl#> .
@prefix rdf: <http://www.w3.org/1999/02/22-rdf-syntax-ns#> .
@prefix rdfs: <http://www.w3.org/2000/01/rdf-schema#> .
@prefix sh-dcat: <http://example.org/shapes/dcat/> .
@prefix skos: <http://www.w3.org/2004/02/skos/core#> .
@prefix time: <http://www.w3.org/2006/time#> .
@prefix uco-core: <https://ontology.unifiedcyberontology.org/uco/core/> .
@prefix uco-observable: <https://ontology.unifiedcyberontology.org/uco/observable/> .
@prefix uco-time: <https://ontology.unifiedcyberontology.org/uco/time/> .
@prefix vcard: <http://www.w3.org/2006/vcard/ns#> .
@prefix xsd: <http://www.w3.org/2001/XMLSchema#> .

<http://example.org/ontology/case-corpora>
	a owl:Ontology ;
	rdfs:comment "This ontology serves to join the versions of CASE and DCAT used to populate CASE-Corpora, bringing analogous properties and classes together."@en ;
	owl:imports
		time:2016 ,
		<http://www.w3.org/2006/vcard/ns> ,
		<http://www.w3.org/ns/dcat> ,
		<http://xmlns.com/foaf/0.1/> ,
		<https://ontology.caseontology.org/case/case/1.1.0>
		;
	.

case-corpora:Catalog
	a owl:Class ;
	rdfs:subClassOf
		case-corpora:Dataset ,
		dcat:Catalog
		;
	.

case-corpora:Dataset
	a owl:Class ;
	rdfs:subClassOf
		dcat:Dataset ,
		uco-core:ContextualCompilation
		;
	skos:editorialNote "Note that by subclassing a uco-core:ContextualCompilation, a case-corpora:Dataset must have at least one distribution associated, due to a uco-core:ContextualCompilation requiring at least one member."@en ;
	.

case-corpora:Distribution
	a owl:Class ;
	rdfs:subClassOf
		dcat:Distribution ,
		uco-observable:ObservableObject
		;
	.

case-corpora:IANAMediaType
	a owl:Class ;
	rdfs:subClassOf dcterms:MediaType ;
	rdfs:comment "This class is provided to satisfy the DCAT requirement that dcat:mediaType's range be 'The media type of the distribution as defined by IANA'.  A dcterms:MediaType is not necessarily a media type defined by IANA; dcterms:format suggests IANA Media Types are one potential media type set."@en ;
	rdfs:seeAlso
		dcterms:format ,
		<https://github.com/ucoProject/UCO/issues/363>
		;
	.

case-corpora:WebPage
	a owl:Class ;
	rdfs:subClassOf
		foaf:Document ,
		uco-observable:WebPage
		;
	rdfs:comment "This class is provided to unify DCAT's range requirement of dcat:landingPage with an appropriate UCO class."@en ;
	.

case-corpora:contact-00000000-0000-0000-0000-000000000000
	a
		vcard:Contact ,
		vcard:Individual
		;
	rdfs:comment "This named individual is provided as a stand-in to make explict that no point of contact is available, linked, or otherwise represented for a dataset."@en ;
	rdfs:seeAlso
		sh-dcat:contactPoint-range-shape ,
		dcat:contactPoint ,
		<https://resources.data.gov/resources/dcat-us/#contactPoint>
		;
	vcard:fn "NOT ENCODED" ;
	vcard:hasEmail <mailto:null@example.org> ;
	.

case-corpora:hasDatasetDirectory
	a owl:DatatypeProperty ;
	rdfs:comment "This property provides an identifier for a dcat:Dataset that is unique within the scope of CASE-Corpora.  Its technical purpose is to keep directory names distinct across the datasets.  Its value is the basename of the directory directly under /catalog/datasets housing the graph source files for the dataset."@en ;
	rdfs:domain dcat:Dataset ;
	rdfs:range xsd:string ;
	.

case-corpora:hasDistribution
	a owl:ObjectProperty ;
	rdfs:subPropertyOf
		dcat:distribution ,
		uco-core:object
		;
	rdfs:domain case-corpora:Dataset ;
	rdfs:range case-corpora:Distribution ;
	.

case-corpora:hasDownloadURL
	a owl:ObjectProperty ;
	rdfs:subPropertyOf dcat:downloadURL ;
	rdfs:domain case-corpora:Distribution ;
	rdfs:range uco-observable:URL ;
	.

<http://purl.org/dc/aboutdcmi#DCMI>
	rdfs:comment "TODO - This is to work around a bug where pyshacl reviewed ontology content instead of data content.  Need to report a test case."@en ;
	skos:prefLabel "" ;
	.

dcat:Dataset
	rdfs:comment "Within CASE-Corpora, the property hasDatasetDirectory is a unique identifier for a Dataset."@en ;
	owl:hasKey case-corpora:hasDatasetDirectory ;
	.

<mailto:null@example.org>
	a vcard:Email ;
	rdfs:comment "This individual is defined to satisfy a DCAT-US constraint."@en ;
	.

